open import Preliminaries

module Lab3-LRSol where

  {- de Bruijn indices are representd as proofs that 
     an element is in a list -}
  data _∈_ {A : Set} : (x : A) (l : List A) → Set where -- type \in
    i0 : {x : A} {xs : List A} → x ∈ x :: xs
    iS : {x y : A} {xs : List A} → x ∈ xs → x ∈ y :: xs

  {- types of the STLC -}
  data Tp : Set where
    b : Tp             -- uninterpreted base type
    _⇒_ : Tp → Tp → Tp -- type \=>

  {- contexts are lists of Tp's -}
  Ctx = List Tp
  _,,_ : Ctx → Tp → Ctx
  Γ ,, τ = τ :: Γ

  infixr 10 _⇒_
  infixr 9 _,,_
  infixr 8 _|-_ -- type \entails

  {- Γ ⊢ τ represents a term of type τ in context Γ -}
  data _|-_ (Γ : Ctx) : Tp → Set where
    c   : Γ |- b -- some constant of the base type
    v   : {τ : Tp} 
        → τ ∈ Γ
        → Γ |- τ 
    lam : {τ1 τ2 : Tp} 
        → Γ ,, τ1 |- τ2
        → Γ |- τ1 ⇒ τ2
    app : {τ1 τ2 : Tp} 
        → Γ |- τ1 ⇒ τ2 
        → Γ |- τ1 
        → Γ |- τ2

  module Examples where
    i : [] |- b ⇒ b
    i = lam (v i0) -- \ x -> x
  
    k : [] |- b ⇒ b ⇒ b
    k = lam (lam (v (iS i0))) -- \ x -> \ y -> x
  
    {- TASK 1: Define a term representing  \ x -> \ y -> y -}
    k' : [] |- b ⇒ b ⇒ b
    k' = lam (lam (v i0))
  

  {- The following proof is like a "0-ary" logical relation.
     It gives a semantics of the STLC in Agda.
     This shows that the STLC is sound, relative to Agda.  
  -}
  module Semantics (B : Set) (elB : B) where 
    -- works for any interpretation of the base type b

    -- function mapping STLC types to Agda types
    [_]t : Tp → Set  -- type \(0 and \)0
    [ b ]t = B
    [ τ1 ⇒ τ2 ]t = [ τ1 ]t → [ τ2 ]t

    -- function mapping STLC contexts to Agda types
    [_]c : Ctx → Set
    [ [] ]c = Unit
    [ τ :: Γ ]c = [ Γ ]c × [ τ ]t

    {- TASK 2 : Define the interpretation of terms -}
    [_] : {Γ : Ctx} {τ : Tp} → Γ |- τ → [ Γ ]c → [ τ ]t
    [ c ] γ = elB
    [ v i0 ] γ = snd γ
    [ v (iS x) ] γ = [ v x ] (fst γ) 
    [ lam e ] γ = \ x → [ e ] (γ , x)
    [ app e1 e2 ] γ = [ e1 ] γ ([ e2 ] γ)

    {- the following test should pass
    test : ⟦ Examples.k ⟧ == \ γ x y → x
    test = Refl
    -}



  {- you can ignore the implementation of this module.
     the interface for the components you need is listed below
  -}
  module RenamingAndSubstitution where 

    -- renamings = variable for variable substitutions.
    -- For simplicity, these are defined as tuples, by recursion on the context.
    -- It might clean up some of the proofs to use a functional view,
    --   {τ : Tp} → τ ∈ Γ → τ ∈ Γ'
    -- because then we could avoid some of the inductions here,
    -- and some of the associativity/unit properties would be free.  
    module Renamings where

      infix 9 _⊇_
  
      _⊇_ : Ctx → Ctx → Set -- type \sup=
      Γ' ⊇ [] = Unit
      Γ' ⊇ (τ :: Γ) = (Γ' ⊇ Γ) × (τ ∈ Γ')

      -- variables are functorial in the context
      rename-var : {Γ Γ' : Ctx} {τ : Tp} → Γ' ⊇ Γ → τ ∈ Γ → τ ∈ Γ'
      rename-var (ρ , x') i0 = x'
      rename-var (ρ , _) (iS x) = rename-var ρ x
  
      {- conceptually, we could define p and ⊇-compose and ⊇-id as primitive
         and derive this.
         but this works better inductively than ⊇-single does.
      -}
      p· : {Γ : Ctx} {Γ' : Ctx} → Γ ⊇ Γ' → {τ : Tp} → (Γ ,, τ) ⊇ Γ'
      p· {Γ' = []} ren = <>
      p· {Γ' = (τ :: Γ')} (ρ , x) = p· ρ , iS x
  
      idr : {Γ : Ctx} → Γ ⊇ Γ
      idr {[]} = <>
      idr {τ :: Γ} = p· idr , i0
  
      _·rr_ : {Γ1 Γ2 Γ3 : Ctx} → Γ1 ⊇ Γ2 → Γ2 ⊇ Γ3 → Γ1 ⊇ Γ3
      _·rr_ {Γ1} {Γ2} {[]} ρ2 ρ3 = <>
      _·rr_ {Γ1} {Γ2} {x :: Γ3} ρ2 (ρ3 , x3) = (ρ2 ·rr ρ3) , rename-var ρ2 x3

      -- category with families notation
      p : {Γ : Ctx} {τ : Tp} → (Γ ,, τ ⊇ Γ) 
      p = p· idr 
      
      -- next, we should show associativity and unit laws for ∘rr.
      -- However:
      -- (1) because renamings are defined using variables, this depends on (some of) functoriality of τ ∈ -,
      --     so we define that here, too.  
      -- (2) we only need one of the unit laws

      rename-var-· : {Γ1 Γ2 Γ3 : Ctx} → (ρ2 : Γ1 ⊇ Γ2) (ρ3 : Γ2 ⊇ Γ3) {τ : Tp} (x : τ ∈ Γ3)
                         → rename-var ρ2 (rename-var ρ3 x) == rename-var (_·rr_ ρ2 ρ3) x
      rename-var-· ρ2 ρ3 i0 = Refl
      rename-var-· ρ2 ρ3 (iS x) = rename-var-· ρ2 (fst ρ3) x

      ·rr-assoc : {Γ1 Γ2 Γ3 Γ4 : Ctx} → (ρ2 : Γ1 ⊇ Γ2) (ρ3 : Γ2 ⊇ Γ3) (ρ4 : Γ3 ⊇ Γ4) → _·rr_ ρ2 (_·rr_ ρ3 ρ4) == _·rr_ (_·rr_ ρ2 ρ3) ρ4 
      ·rr-assoc {Γ4 = []} ρ2 ρ3 ρ4 = Refl
      ·rr-assoc {Γ4 = τ4 :: Γ4} ρ2 ρ3 (ρ4 , x4) = ap2 _,_ (·rr-assoc ρ2 ρ3 ρ4) (rename-var-· ρ2 ρ3 x4)

      -- rest of functoriality of rename-var
      mutual
        -- generalization to get the induction to go through
        rename-var-p' : {Γ Γ' : Ctx} {τ τ' : Tp} (ρ : Γ' ⊇ Γ) (x : τ ∈ Γ) → rename-var (p· ρ {τ'}) x == (iS (rename-var ρ x))
        rename-var-p' ρ i0 = Refl
        rename-var-p' (ρ , _) (iS x) = rename-var-p' ρ x
  
        -- this would be definitional if renamings were functions.
        -- this instances is often needed below
        rename-var-p : {Γ : Ctx} {τ τ' : Tp} (x : τ ∈ Γ) → rename-var (p· idr {τ'}) x == (iS x)
        rename-var-p x = ap iS (rename-var-ident _ x) ∘ rename-var-p' idr x

        rename-var-ident : {τ : Tp} (Γ : Ctx) (x : τ ∈ Γ) → rename-var idr x == x
        rename-var-ident .(τ :: Γ) (i0 {τ} {Γ}) = Refl
        rename-var-ident .(τ' :: Γ) (iS {τ} {τ'} {Γ} x) = rename-var-p x

      -- beta reduction for p
      pβ1' : {Γ1 Γ2 Γ3 : Ctx} → (ρ2 : Γ1 ⊇ Γ2) (ρ3 : Γ2 ⊇ Γ3) {τ : Tp} (x : τ ∈ Γ1)
            → (ρ2 , x) ·rr (p· ρ3) == (ρ2 ·rr ρ3)
      pβ1' {Γ1} {_} {[]} ρ2 ρ3 x = Refl
      pβ1' {Γ1} {_} {τ3 :: Γ3} ρ2 (ρ3 , x3) x₁ = ap (λ x → x , rename-var ρ2 x3) (pβ1' ρ2 ρ3 _)

      mutual
        ·rr-unitr : {Γ1 Γ2 : Ctx} → (ρ2 : Γ1 ⊇ Γ2) 
              → ρ2 ·rr idr == ρ2
        ·rr-unitr {Γ1} {[]} ρ2 = Refl
        ·rr-unitr {Γ1} {τ2 :: Γ2} (ρ2 , x2) = ap (λ x → x , x2) (pβ1 ρ2 x2)
  
        pβ1 : {Γ1 Γ2 : Ctx} → (ρ2 : Γ1 ⊇ Γ2) {τ : Tp} (x : τ ∈ Γ1)
              → (ρ2 , x) ·rr p == ρ2
        pβ1 ρ2 x = ·rr-unitr ρ2 ∘ pβ1' ρ2 idr x

      -- p· is equivalent to the alternate definition.
      p·-def : {Γ1 Γ2 : Ctx} {τ : Tp} (ρ : Γ1 ⊇ Γ2) → p· ρ {τ} == p ·rr ρ
      p·-def {_}{[]} ρ = Refl
      p·-def {_}{τ1 :: Γ1} (ρ , x) = ap2 _,_ (p·-def ρ) (! (rename-var-p x))


      -- terms are functorial in renamings

      addvar-ren : {Γ Γ' : Ctx} {τ : Tp} → Γ' ⊇ Γ → Γ' ,, τ ⊇ Γ ,, τ
      addvar-ren ρ = (p· ρ , i0)
  
      rename : {Γ Γ' : Ctx} {τ : Tp} → Γ' ⊇ Γ → Γ |- τ → Γ' |- τ
      rename ρ c = c
      rename ρ (v x) = v (rename-var ρ x)
      rename ρ (lam e) = lam (rename (addvar-ren ρ) e)
      rename ρ (app e e') = app (rename ρ e) (rename ρ e')

      rename-· : {Γ1 Γ2 Γ3 : Ctx} → (ρ2 : Γ1 ⊇ Γ2) (ρ3 : Γ2 ⊇ Γ3) {τ : Tp} (e : Γ3 |- τ)
                     → rename ρ2 (rename ρ3 e) == rename (ρ2 ·rr ρ3) e
      rename-· ρ2 ρ3 c = Refl
      rename-· ρ2 ρ3 (v x) = ap v (rename-var-· ρ2 ρ3 x)
      rename-·{Γ1}{Γ2}{Γ3} ρ2 ρ3 (lam e) = ap lam (ap (λ x → rename (x , i0) e) lemma1 ∘ rename-· (addvar-ren ρ2) (addvar-ren ρ3) e) where
        lemma1 : (p· ρ2 , i0) ·rr (p· ρ3) == p· (ρ2 ·rr ρ3)
        lemma1 = (p· ρ2 , i0) ·rr (p· ρ3)  =⟨ pβ1' (p· ρ2) ρ3 i0 ⟩
                 (p· ρ2) ·rr ρ3            =⟨ ap (λ x → _·rr_ x ρ3) (p·-def ρ2) ⟩
                 (p ·rr ρ2) ·rr ρ3         =⟨ ! (·rr-assoc p ρ2 ρ3) ⟩ 
                 p ·rr (ρ2 ·rr ρ3)         =⟨ ! (p·-def (ρ2 ·rr ρ3))⟩
                 p· (ρ2 ·rr ρ3) ∎
      rename-· ρ2 ρ3 (app e e₁) = ap2 app (rename-· ρ2 ρ3 e) (rename-· ρ2 ρ3 e₁)

      -- not necessary for the proof, but an easy corollary of the above
      rename-id : {Γ : Ctx}{τ : Tp} (e : Γ |- τ) → rename idr e == e
      rename-id c = Refl
      rename-id (v x) = ap v (rename-var-ident _ x)
      rename-id (lam e) = ap lam (rename-id e)
      rename-id (app e e₁) = ap2 app (rename-id e) (rename-id e₁)
    open Renamings

    -- expression-for-variable substitutions

    module Subst where

      _|-c_ : Ctx → Ctx → Set
      Γ' |-c [] = Unit
      Γ' |-c (τ :: Γ) = (Γ' |-c Γ) × (Γ' |- τ) 
  
      _·rs_ : {Γ1 Γ2 Γ3 : Ctx} →  Γ1 ⊇ Γ2 → Γ2 |-c Γ3 → Γ1 |-c Γ3
      _·rs_ {Γ1} {Γ2} {[]} ρ θ = <>
      _·rs_ {Γ1} {Γ2} {τ3 :: Γ3} ρ (θ , e) = ρ ·rs θ , rename ρ e
    
      addvar : {Γ Γ' : Ctx} {τ : Tp} → Γ |-c Γ' → (Γ ,, τ) |-c (Γ' ,, τ)
      addvar θ = p ·rs θ , v i0
  
      ids : {Γ : Ctx} → Γ |-c Γ
      ids {[]} = <>
      ids {τ :: Γ} = p ·rs ids , v i0
  
      subst-var : {Γ Γ' : Ctx}{τ : Tp} → Γ |-c Γ' → τ ∈ Γ' → Γ |- τ
      subst-var (θ , e) i0 = e
      subst-var (θ , _) (iS x) = subst-var θ x

      subst : {Γ Γ' : Ctx}{τ : Tp} → Γ |-c Γ' → Γ' |- τ  → Γ |- τ
      subst θ c = c
      subst θ (v x) = subst-var θ x
      subst θ (lam e) = lam (subst (addvar θ) e)
      subst θ (app e e') = app (subst θ e) (subst θ e')
  
      subst1 : {τ τ0 : Tp} → [] |- τ0 → ([] ,, τ0) |- τ → [] |- τ
      subst1 e0 e = subst (<> , e0) e


      -- composition of renamings and substitutions

      _·sr_ : {Γ1 Γ2 Γ3 : Ctx} →  Γ1 |-c Γ2 → Γ2 ⊇ Γ3 → Γ1 |-c Γ3
      _·sr_ {Γ1} {Γ2} {[]} θ ρ = <>
      _·sr_ {Γ1} {Γ2} {τ3 :: Γ3} θ (ρ , x) = _·sr_ θ ρ , subst-var θ x

      _·ss_ : {Γ1 Γ2 Γ3 : Ctx} → Γ1 |-c Γ2 → Γ2 |-c Γ3 → Γ1 |-c Γ3
      _·ss_ {Γ3 = []} θ1 θ2 = <>
      _·ss_ {Γ1} {Γ2} {τ :: Γ3} θ1 (θ2 , e2) = θ1 ·ss θ2 , subst θ1 e2

  
      -- subst var functoriality

      subst-var-·rs : {Γ1 Γ2 Γ3 : Ctx} (ρ : Γ1 ⊇ Γ2) (θ : Γ2 |-c Γ3) {τ : Tp} (x : τ ∈ Γ3)
                           → subst-var (ρ ·rs θ) x == rename ρ (subst-var θ x)
      subst-var-·rs ρ θ i0 = Refl
      subst-var-·rs ρ (θ , _) (iS x) = subst-var-·rs ρ θ x

      subst-var-∘ss : {Γ1 Γ2 Γ3 : Ctx} → (θ2 : Γ1 |-c Γ2) (θ3 : Γ2 |-c Γ3) {τ : Tp} (x : τ ∈ Γ3)
                        → subst-var (_·ss_ θ2 θ3) x == subst θ2 (subst-var θ3 x)
      subst-var-∘ss θ2 θ3 i0 = Refl
      subst-var-∘ss θ2 (θ3 , _) (iS x) = subst-var-∘ss θ2 θ3 x

      subst-var-·sr : {Γ1 Γ2 Γ3 : Ctx} {τ : Tp} → (θ2 : Γ1 |-c Γ2) (ρ : Γ2 ⊇ Γ3) (x : τ ∈ Γ3)
                           → (subst-var θ2 (rename-var ρ x)) == subst-var (_·sr_ θ2 ρ) x
      subst-var-·sr θ2 ρ i0 = Refl
      subst-var-·sr θ2 ρ (iS x) = subst-var-·sr θ2 (fst ρ) x

      subst-var-id : {Γ : Ctx} {τ : Tp} → (x : τ ∈ Γ) → v x == subst-var ids x
      subst-var-id i0 = Refl
      subst-var-id {τ :: Γ} (iS x) = !
        (_ =〈 subst-var-·rs (p· idr) ids x 〉
         rename (p· idr) _ =〈 ! (ap (rename (p· idr)) (subst-var-id x)) 〉
         rename (p· idr) (v x) =〈 ap v (rename-var-p x) 〉
         v (iS x) ∎)


      -- associativity and unit laws for composition.
      -- also includes some β rules for composing with p.
      -- and functoriality of subst in the various compositions, since substitutions involve terms.

      ∘rsr-assoc : {Γ1 Γ2 Γ3 Γ4 : Ctx} → (ρ2 : Γ1 ⊇ Γ2) (θ3 : Γ2 ⊢c Γ3) (ρ4 : Γ3 ⊇ Γ4)
                 → (ρ2 ·rs θ3) ·sr ρ4 == ρ2 ·rs (θ3 ·sr ρ4)
      ∘rsr-assoc {Γ1} {Γ2} {Γ3} {[]} ρ2 θ3 ρ4 = Refl
      ∘rsr-assoc {Γ1} {Γ2} {Γ3} {τ4 :: Γ4} ρ2 θ3 (ρ4 , x4) = ap2 _,_ (∘rsr-assoc ρ2 θ3 ρ4) (subst-var-·rs ρ2 θ3 x4)

      ·sr-pβ'  : {Γ1 Γ2 Γ3 : Ctx} {τ : Tp} → (θ2 : Γ1 ⊢c Γ2) (ρ : Γ2 ⊇ Γ3) {e : _ ⊢ τ}
                → (θ2 , e) ·sr (p· ρ) == θ2 ·sr ρ
      ·sr-pβ' {Γ1} {Γ2} {[]} θ2 ρ = Refl
      ·sr-pβ' {Γ1} {Γ2} {τ :: Γ3} θ2 (ρ , x) = ap2 _,_ (·sr-pβ' θ2 ρ) Refl

      mutual
        ·sr-unitr : {Γ1 Γ2 : Ctx} → (θ : Γ1 ⊢c Γ2) → θ ·sr idr == θ
        ·sr-unitr {Γ1} {[]} θ = Refl
        ·sr-unitr {Γ1} {τ2 :: Γ2} (θ , e) = ap (λ x → x , e) (·sr-pβ θ)
  
        ·sr-pβ  : {Γ1 Γ2 : Ctx} {τ : Tp} → (θ2 : Γ1 ⊢c Γ2) {e : _ ⊢ τ}
                         → (θ2 , e) ·sr p == θ2
        ·sr-pβ θ2 = ·sr-unitr θ2 ∘ ·sr-pβ' θ2 idr

      subst-id : {Γ : Ctx} {τ : Tp} {e : Γ ⊢ τ} → e == subst (ids) e 
      subst-id {e = c} = Refl
      subst-id {e = v x} = subst-var-id x
      subst-id {e = lam e} = ap lam (subst-id)
      subst-id {e = app e e₁} = ap2 app subst-id subst-id 

      subst-·rs : {Γ1 Γ2 Γ4 : Ctx} {τ : Tp} → (ρ : Γ4 ⊇ Γ1) (θ2 : Γ1 ⊢c Γ2) (e : Γ2 ⊢ τ)
                → rename ρ (subst θ2 e) == subst (ρ ·rs θ2) e
      subst-·rs ρ θ2 c = Refl
      subst-·rs ρ θ2 (v x) = ! (subst-var-·rs ρ θ2 x)
      subst-·rs ρ θ2 (lam e) = ap lam (ap (λ x → subst x e) (ap (λ x → x , v i0) (lemma2 ρ θ2)) ∘ subst-·rs (addvar-ren ρ) (addvar θ2) e) where
              lemma1 : {Γ3 Γ5 : Ctx} (ρ₁ : Γ5 ⊇ Γ3) {τ3 : Tp}
                     →  (addvar-ren {_}{_}{τ3} ρ₁) ·rr (p· idr) == (p· idr) ·rr ρ₁
              lemma1 {Γ3} {Γ5} ρ₁ = (p· ρ₁ , i0) ·rr (p· idr) =〈 Refl 〉
                                   (p· ρ₁ , i0) ·rr  p       =〈 ap (λ x → (x , i0) ·rr p) (p·-def ρ₁)〉 
                                   (p ·rr ρ₁ , i0) ·rr  p    =〈 pβ1 (p ·rr ρ₁) i0 〉 
                                   p ·rr ρ₁                  =〈 Refl 〉
                                   (p· idr) ·rr ρ₁ ∎

              lemma2 : {Γ1 Γ2 Γ4 : Ctx} {τ : Tp} → (ρ : Γ4 ⊇ Γ1) (θ2 : Γ1 ⊢c Γ2) 
                     → (addvar-ren{_}{_}{τ} ρ) ·rs (fst (addvar θ2)) == p ·rs (ρ ·rs θ2)
              lemma2 {Γ2 = []} ρ₁ θ3 = Refl
              lemma2 {Γ2 = τ2 :: Γ2} ρ₁ (θ3 , e3) = ap2 _,_ (lemma2 ρ₁ θ3) 
                         (! (rename-· (p·  idr) ρ₁ e3) ∘ 
                          (ap (λ x → rename x e3) (lemma1 ρ₁) ∘ 
                           rename-· (addvar-ren ρ₁) (p·  idr) e3))
      subst-·rs ρ θ2 (app e e₁) = ap2 app (subst-·rs ρ θ2 e) (subst-·rs ρ θ2 e₁) 

      ·rss-assoc : {Γ1 Γ2 Γ3 Γ4 : Ctx} → (ρ : Γ4 ⊇ Γ1) (θ2 : Γ1 ⊢c Γ2) (θ3 : Γ2 ⊢c Γ3)
                           → ρ ·rs (θ2 ·ss θ3) == (ρ ·rs θ2) ·ss θ3
      ·rss-assoc {Γ1} {Γ2} {[]} ρ θ2 θ3 = Refl
      ·rss-assoc {Γ1} {Γ2} {x :: Γ3} ρ θ2 (θ3 , e3) = ap2 _,_ (·rss-assoc ρ θ2 θ3) (subst-·rs ρ θ2 e3)

      subst-·sr : {Γ1 Γ2 Γ3 : Ctx} {τ : Tp} → (θ2 : Γ1 ⊢c Γ2) (ρ : Γ2 ⊇ Γ3) (e : Γ3 ⊢ τ)
                           → (subst θ2 (rename ρ e)) == subst (θ2 ·sr ρ) e
      subst-·sr θ2 ρ c = Refl
      subst-·sr θ2 ρ (v x) = subst-var-·sr θ2 ρ x
      subst-·sr θ2 ρ (lam e) = ap lam (ap (λ x → subst x e) (ap (λ x → x , v i0) (lemma θ2 ρ)) ∘ subst-·sr (addvar θ2) (addvar-ren ρ) e) where
         lemma :  {Γ1 Γ2 Γ3 : Ctx} {τ : Tp} → (θ2 : Γ1 ⊢c Γ2) (ρ : Γ2 ⊇ Γ3) → (addvar{_}{_}{τ} θ2) ·sr (p· ρ) == p ·rs (θ2 ·sr ρ)
         lemma θ2 ρ = ∘rsr-assoc (p·  idr) θ2 ρ ∘ ·sr-pβ' (_·rs_ (p·  idr) θ2) ρ {v i0}
      subst-·sr θ2 ρ (app e e₁) = ap2 app (subst-·sr θ2 ρ e) (subst-·sr θ2 ρ e₁) 

      ·srs-assoc : {Γ1 Γ2 Γ3 Γ4 : Ctx} (θ : Γ1 ⊢c Γ2) (ρ : Γ2 ⊇ Γ3) (θ' : Γ3 ⊢c Γ4) 
                 → θ ·ss (ρ ·rs θ') == (θ ·sr ρ) ·ss θ'
      ·srs-assoc {Γ1} {Γ2} {Γ3} {[]} θ ρ θ' = Refl
      ·srs-assoc {Γ1} {Γ2} {Γ3} {x :: Γ4} θ ρ (θ' , e') = ap2 _,_ (·srs-assoc θ ρ θ') (subst-·sr θ ρ e')

      subst-·ss : {Γ1 Γ2 Γ3 : Ctx} → (θ2 : Γ1 ⊢c Γ2) (θ3 : Γ2 ⊢c Γ3) {τ : Tp} (e : Γ3 ⊢ τ)
                    → subst (θ2 ·ss θ3) e == subst θ2 (subst θ3 e)
      subst-·ss θ2 θ3 c = Refl
      subst-·ss θ2 θ3 (v x) = subst-var-∘ss θ2 θ3 x
      subst-·ss θ2 θ3 (lam e) = ap lam (subst-·ss (addvar θ2) (addvar θ3) e ∘ 
                                            ap (λ x → subst x e) (ap (λ x → x , v i0) 
                                               (lemma1 ∘ ·rss-assoc p θ2 θ3))) where
                    lemma1 : (p ·rs θ2) ·ss θ3 ==
                             (addvar θ2) ·ss (fst (addvar θ3))
                    lemma1 = (p ·rs θ2) ·ss θ3 =〈 ! (ap (λ x → x ·ss θ3) (·sr-pβ (p ·rs θ2) {v i0})) 〉 
                             ((p ·rs θ2 , v i0) ·sr p) ·ss θ3 =〈 ! (·srs-assoc (p ·rs θ2 , v i0) p θ3) 〉
                             (p ·rs θ2 , v i0) ·ss (p ·rs θ3) ∎
      subst-·ss θ2 θ3 (app e e₁) = ap2 app (subst-·ss θ2 θ3 e) (subst-·ss θ2 θ3 e₁)

      ·ss-unitl : {Γ1 Γ2 : Ctx} → (θ : Γ1 ⊢c Γ2) → ids ·ss θ == θ
      ·ss-unitl {Γ2 = []} θ = Refl
      ·ss-unitl {Γ2 = τ :: Γ2} (θ , e) = ap2 _,_ (·ss-unitl θ) (! subst-id)

      compose1 : {τ1 τ2 : Tp} {Γ : Ctx} (θ : [] ⊢c Γ) (e' : [] ⊢ τ1) 
               → (θ , e') == (<> , e') ·ss (addvar θ)
      compose1 {τ1}{τ2} θ e' = ap (λ x → x , e') (! (·srs-assoc (<> , e') (p{_}{τ1}) θ) ∘ ! (·ss-unitl θ))

      subst-compose1 : {τ1 τ2 : Tp} {Γ : Ctx} (θ : [] ⊢c Γ) (e' : [] ⊢ τ1) (e : Γ ,, τ1 ⊢ τ2)
              → subst (θ , e') e == subst1 e' (subst (addvar θ) e)
      subst-compose1{τ1}{τ2}{Γ} θ e' e = subst-·ss (<> , e') (addvar θ) e ∘ ap (λ x → subst x e) (compose1{τ1}{τ2}{Γ} θ e')

    open Subst public

  open RenamingAndSubstitution using (subst1 ; _⊢c_ ; subst ; subst-id ; subst-compose1)
  {- θ : Γ ⊢c Γ' means θ is a substitution for Γ' in terms of Γ.  It is defined as follows:

    _⊢c_ : Ctx → Ctx → Set
    Γ' ⊢c [] = Unit
    Γ' ⊢c (τ :: Γ) = (Γ' ⊢c Γ) × (Γ' ⊢ τ) 

    -- apply a substitution to a term
    subst : {Γ Γ' : Ctx}{τ : Tp} → Γ ⊢c Γ' → Γ' ⊢ τ  → Γ ⊢ τ

    -- substitution for a single variable
    subst1 : {τ τ0 : Tp} → [] ⊢ τ0 → ([] ,, τ0) ⊢ τ → [] ⊢ τ

    -- you will need these two properties:
    subst-compose1 : {τ1 τ2 : Tp} {Γ : Ctx} (θ : [] ⊢c Γ) (e' : [] ⊢ τ1) (e : Γ ,, τ1 ⊢ τ2)
                   → subst (θ , e') e == subst1 e' (subst (addvar θ) e)

    subst-id : {Γ : Ctx} {τ : Tp} {e : Γ ⊢ τ} → e == subst (ids) e 
  -}

  
  module OpSem where
    -- step relation
    data _↦_ : {τ : Tp} → [] |- τ → [] |- τ → Set where
      Step/app  :{τ1 τ2 : Tp} {e e' : [] |- τ1 ⇒ τ2} {e1 : [] |- τ1}
             → e ↦ e'
             → (app e e1) ↦ (app e' e1)
      Step/β : {τ1 τ2 : Tp} {e : [] ,, τ1 |- τ2} {e1 : [] |- τ1}
             → (app (lam e) e1) ↦ subst1 e1 e 

    -- reflexive/transitive closure
    data _↦*_ : {τ : Tp} → [] |- τ → [] |- τ → Set where
      Done : {τ : Tp} {e : [] |- τ} → e ↦* e
      Step : {τ : Tp} {e1 e2 e3 : [] |- τ} 
           → e1 ↦ e2  →  e2 ↦* e3
           → e1 ↦* e3

  {- Next, you will prove "very weak normalization".  The theorem is
     that any closed term *of base type b* evaluates to the constant c.
     No claims are made about terms of function type.
  -}
  module VeryWeakNormalization where

    open OpSem

    WN : (τ : Tp) → [] ⊢ τ → Set
    -- WN_τ(e) iff e ↦* c
    WN b e = e ↦* c
    -- WN_τ(e) iff for all e1 : τ1, if WN_τ1(e1) then WN_τ2(e e1)
    WN (τ1 ⇒ τ2) e = (e1 : [] ⊢ τ1) → WN τ1 e1 → WN τ2 (app e e1)

    -- extend WN to contexts and substitutions
    WNc : (Γ : Ctx) → [] ⊢c Γ → Set
    WNc [] θ = Unit
    WNc (τ :: Γ) (θ , e) = WNc Γ θ × WN τ e

    {- TASK 3 : show that the relation is closed under head expansion: -}
    head-expand : (τ : Tp) {e e' : [] ⊢ τ} → e ↦ e' → WN τ e' → WN τ e
    head-expand b e↦e' w = Step e↦e' w
    head-expand (τ1 ⇒ τ2) e↦e' w = λ e1 we1 → head-expand τ2 (Step/app e↦e') (w e1 we1)

    {- TASK 4 : prove the fundamental theorem -}
    fund : {Γ : Ctx} {τ : Tp} {θ : [] ⊢c Γ} 
         → (e : Γ ⊢ τ)
         → WNc Γ θ 
         → WN τ (subst θ e)
    fund c wθ = Done
    fund (v i0) (_ , we) = we
    fund (v (iS x)) (wθ , _) = fund (v x) wθ
    fund {_}{._}{θ} (lam{τ1}{τ2} e) wθ = 
      λ e1 we1 → head-expand τ2 Step/β
        (transport (λ x → WN τ2 x) (subst-compose1 θ e1 e) (fund e (wθ , we1)))
    fund (app e e₁) wθ = fund e wθ _ (fund e₁ wθ)

    {- TASK 5 : conclude weak normalization at base type -}
    corollary : (e : [] ⊢ b) → e ↦* c
    corollary e = transport (\ x -> x ↦* _) (! subst-id) (fund e <>)


  {- TASK 6 : change the definition of the logical relation so that you also can conclude normalization 
              at function type 
  -}
  module WeakNormalization where

    open OpSem

    WN : (τ : Tp) → [] ⊢ τ → Set
    WN b e = e ↦* c
    WN (τ1 ⇒ τ2) e = 
      Σ \ (e' : [] ,, τ1 ⊢ τ2) → 
      (e ↦* lam e') × ((e1 : [] ⊢ τ1) → WN τ1 e1 → WN τ2 (subst1 e1 e'))

    -- extend WN to contexts and substitutions
    WNc : (Γ : Ctx) → [] ⊢c Γ → Set
    WNc [] θ = Unit
    WNc (τ :: Γ) (θ , e) = WNc Γ θ × WN τ e

    open RenamingAndSubstitution using (addvar)
    --- you will want to use
    --    addvar : {Γ Γ' : Ctx} {τ : Tp} → Γ ⊢c Γ' → (Γ ,, τ) ⊢c (Γ' ,, τ)

    head-expand : (τ : Tp) {e e' : [] ⊢ τ} → e ↦ e' → WN τ e' → WN τ e
    head-expand b e↦e' w = Step e↦e' w
    head-expand (τ1 ⇒ τ2) e↦e' (body , steps , wn) = body , Step e↦e' steps , wn

    -- Hint: you will need a couple of lemmas about ↦* that we didn't need above
    -- (I used three of them)

    head-expand* : {τ : Tp} {e e' : [] ⊢ τ} → e ↦* e' → WN τ e' → WN τ e
    head-expand* Done w = w
    head-expand* (Step s ss) w = head-expand _ s (head-expand* ss w)

    Step/app*  :{τ1 τ2 : Tp} {e e' : [] ⊢ τ1 ⇒ τ2} {e1 : [] ⊢ τ1}
             → e ↦* e'
             → (app e e1) ↦* (app e' e1)
    Step/app* Done = Done
    Step/app* (Step s ss) = (Step (Step/app s) (Step/app* ss))

    Step' : {τ : Tp} {e1 e2 e3 : [] ⊢ τ} 
           → e1 ↦* e2  →  e2 ↦ e3
           → e1 ↦* e3
    Step' Done s = Step s Done
    Step' (Step s ss) s' = Step s (Step' ss s')

    fund : {Γ : Ctx} {τ : Tp} {θ : [] ⊢c Γ} 
         → (e : Γ ⊢ τ)
         → WNc Γ θ 
         → WN τ (subst θ e)
    fund c wθ = Done
    fund (v i0) (_ , we) = we
    fund (v (iS x)) (wθ , _) = fund (v x) wθ
    fund {_}{._}{θ} (lam{τ1}{τ2} e) wθ = 
      subst (addvar θ) e , Done , (λ e1 we1 → transport (WN τ2) (subst-compose1 θ e1 e) (fund e (wθ , we1)))
    fund (app e e₁) wθ with fund e wθ
    ... | (body , reduction , wn) = head-expand* (Step' (Step/app* reduction) Step/β) (wn _ (fund e₁ wθ))

    {- TASK 6a -}
    corollary1 : (e : [] ⊢ b) → e ↦* c 
    corollary1 e = transport (λ x → x ↦* _) (! subst-id) (fund e <>)

    {- TASK 6b -}
    corollary2 : {τ1 τ2 : Tp} (e : [] ⊢ τ1 ⇒ τ2) → Σ \(e' : _) → e ↦* (lam e')
    corollary2 e with (fund e <>)
    ... | (e' , steps , _) = e' , transport (λ x → x ↦* _) (! subst-id) steps
